# 23

$(A,b) = \left(\begin{array}{rrrrr} -2 & 8 & 0 & -4 & 6 \\ 3 & -7 & -5 & 6 & 1 \\ -4 & 8 & 2 & -5 & 2 \\ 2 & 6 & -2 & -2 & 5 \end{array}\right)$

$-0.5 \cdot I = I$

$\longrightarrow \left(\begin{array}{rrrrr} 1 & -4 & 0 & 2 & -3 \\ 3 & -7 & -5 & 6 & 1 \\ -4 & 8 & 2 & -5 & 2 \\ 2 & 6 & -2 & -2 & 5 \end{array}\right)$

$-3 \cdot I + II = II$

$4 \cdot I + III = III$

$-2 \cdot I + IV = IV$

$\longrightarrow \left(\begin{array}{rrrrr} 1 & -4 & 0 & 2 & -3 \\ 0 & 5 & -5 & 0 & 10 \\ 0 & -8 & 2 & 3 & -10 \\ 0 & 14 & -2 & -6 & 11 \end{array}\right)$

$0.2 \cdot II = II$

$\longrightarrow \left(\begin{array}{rrrrr} 1 & -4 & 0 & 2 & -3 \\ 0 & 1 & -1 & 0 & 2 \\ 0 & -8 & 2 & 3 & -10 \\ 0 & 14 & -2 & -6 & 11 \end{array}\right)$

$8 \cdot II + III = III$

$-14 \cdot II + IV = IV$

$\longrightarrow \left(\begin{array}{rrrrr} 1 & -4 & 0 & 2 & -3 \\ 0 & 1 & -1 & 0 & 2 \\ 0 & 0 & -6 & 3 & 6 \\ 0 & 0 & 12 & -6 & -17 \end{array}\right)$

$-\frac 16 \cdot III = III$

$\longrightarrow \left(\begin{array}{rrrrr} 1 & -4 & 0 & 2 & -3 \\ 0 & 1 & -1 & 0 & 2 \\ 0 & 0 & 1 & -\frac 12 & -1 \\ 0 & 0 & 12 & -6 & -17 \end{array}\right)$

$-12 \cdot III + IV = IV$

$\longrightarrow \left(\begin{array}{rrrrr} 1 & -4 & 0 & 2 & -3 \\ 0 & 1 & -1 & 0 & 2 \\ 0 & 0 & 1 & -\frac 12 & -1 \\ 0 & 0 & 0 & 0 & -5 \end{array}\right)$

$n = 4$

$rg(A) = 3$

$rg(A,b) = 4$

$rg(A) < n \land rg(A) \neq rg(A,b) \Rightarrow Ax = b$ ist nicht lÃ¶sbar